coq/ModuleAssumptions.v
@@ -78,11 +78,11 @@ Inductive is_supported_exp : llvm_exp -> Prop :=
       is_supported_conv conv ->
       is_supported_exp e ->
       is_supported_exp (OP_Conversion conv t1 e t2)
-  | IS_OP_Select : forall cond t1 e1 t2 e2,
+  | IS_OP_Select : forall cond t e1 e2,
       is_supported_exp cond ->
       is_supported_exp e1 ->
       is_supported_exp e2 ->
-      is_supported_exp (OP_Select (TYPE_I 1) cond t1 e1 t2 e2)
+      is_supported_exp (OP_Select (TYPE_I 1) cond t e1 t e2)
 .
 
 Inductive is_supported_function_arg : function_arg -> Prop :=
